WIP commit

VCVio/OracleComp/SimSemantics/QueryTracking/LoggingOracle.lean
@@ -4,13 +4,27 @@ Released under Apache 2.0 license as described in the file LICENSE.
 Authors: Devon Tuma
 -/
 import VCVio.OracleComp.SimSemantics.IsTracking
+import VCVio.OracleComp.Coercions.SimOracle
 
 /-!
 # Logging Queries Made by a Computation
 
 -/
 
-variable {ι : Type} [DecidableEq ι] {spec : OracleSpec ι} {α β : Type}
+variable {ι : Type} {spec : OracleSpec ι} {α β : Type}
+
+variable {ι₁ ι₂ : Type} {spec₁ : OracleSpec ι₁} {spec₂ : OracleSpec ι₂}
+
+theorem oracleComp_prod (oa : OracleComp spec (α × β)) :
+    Prod.mk <$> (Prod.fst <$> oa) <*> (Prod.snd <$> oa) = oa := by
+  simp [seq_map_assoc, seq_eq_bind_map]
+  simp [Function.comp_def]
+  sorry
+
+@[ext]
+theorem prod_ext {oa oa' : OracleComp spec (α × β)} (h1 : Prod.fst <$> oa = Prod.fst <$> oa')
+    (h2 : Prod.snd <$> oa = Prod.snd <$> oa') : oa = oa' := by
+  rw [← oracleComp_prod oa, ← oracleComp_prod oa', h1, h2]
 
 namespace OracleSpec
 
@@ -21,7 +35,21 @@ def QueryLog (spec : OracleSpec ι) : Type :=
 
 instance : EmptyCollection (QueryLog spec) := ⟨λ _ ↦ []⟩
 
+-- instance [spec.DecidableEq] : DecidableEq (QueryLog spec) where
+--   decide x y := by sorry
+
 namespace QueryLog
+
+@[ext]
+theorem ext (log₁ log₂ : QueryLog spec) (h : ∀ i, log₁ i = log₂ i) : log₁ = log₂ := by
+  unfold QueryLog
+  ext i : 1
+  exact h i
+
+@[simp]
+theorem emptyCollection_eq : (∅ : QueryLog spec) = λ _ ↦ [] := rfl
+
+variable [DecidableEq ι] [DecidableEq ι₁] [DecidableEq ι₂]
 
 section logQuery
 
@@ -40,11 +68,41 @@ def wasQueried [spec.DecidableEq] (log : QueryLog spec) (i : ι) (t : spec.domai
   | Option.some _ => true
   | Option.none => false
 
+-- Note: `List.eraseDup(s)` should be the right function (remove all but the first occurrence),
+-- while `dedup` removes all but the last occurrence. However there's not as many supporting lemmas
+-- for `eraseDup` right now.
+def append [spec.DecidableEq] (log₁ : QueryLog spec) (log₂ : QueryLog spec) : QueryLog spec :=
+  λ i ↦ (log₁ i ++ log₂ i).dedup
+
+section Append
+
+def fst (log : QueryLog (spec₁ ++ₒ spec₂)) : QueryLog spec₁ :=
+  λ i ↦ log (.inl i)
+def snd (log : QueryLog (spec₁ ++ₒ spec₂)) : QueryLog spec₂ :=
+  λ i ↦ log (.inr i)
+
+def inl (log : QueryLog spec₁) : QueryLog (spec₁ ++ₒ spec₂)
+  | .inl i => log i | .inr _ => []
+def inr (log : QueryLog spec₂) : QueryLog (spec₁ ++ₒ spec₂)
+  | .inl _ => [] | .inr i => log i
+
+instance : Coe (QueryLog spec₁) (QueryLog (spec₁ ++ₒ spec₂)) := ⟨inl⟩
+instance : Coe (QueryLog spec₂) (QueryLog (spec₁ ++ₒ spec₂)) := ⟨inr⟩
+
+theorem append_empty [spec.DecidableEq] (log : QueryLog spec) (h : ∀ i, (log i).Nodup) :
+    log.append ∅ = log := by
+  ext i : 1
+  simp [append, List.dedup_eq_self, h]
+
+end Append
+
 end QueryLog
 
 end OracleSpec
 
 open OracleComp OracleSpec
+
+variable [DecidableEq ι] [DecidableEq ι₁] [DecidableEq ι₂]
 
 /-- Simulation oracle for tracking the quries in a `QueryLog`, without modifying the actual
 behavior of the oracle. Requires decidable equality of the indexing set to determine
@@ -62,7 +120,40 @@ lemma apply_eq (q : OracleQuery spec α) : loggingOracle.impl q =
       let u ← query i t
       modifyGet λ log ↦ (u, log.logQuery t u)) := rfl
 
+-- May need `SatisfiesM` machinery since the `QueryLog` is inside `OracleComp`
+-- lemma nodup_logQuery (oa : OracleComp spec α) : ∀ i, (simulate loggingOracle ∅ oa).Nodup := by
+
 instance : (loggingOracle (spec := spec)).IsTracking where
   state_indep | query _ _, _ => rfl
+
+theorem simulate_eq_append_simulate_empty [spec.DecidableEq] (oa : OracleComp spec α)
+    (log : QueryLog spec) :
+      simulate loggingOracle log oa = do
+        let ⟨a, log_oa⟩ ← simulate loggingOracle ∅ oa
+        return (a, log.append log_oa) := by
+  induction oa using OracleComp.induction with
+  | pure a => simp [simulate_pure]; ext : 1; simp [QueryLog.append]; sorry
+  | query_bind i t oa ih => simp [simulate_bind, ih]; sorry
+  | failure => simp
+
+-- TODO: add lemmas about behavior of `loggingOracle`
+#check List.eraseDups
+
+variable [spec₁.DecidableEq] [spec₂.DecidableEq]
+
+-- Should this be `simp`?
+theorem inl_eq (oa : OracleComp spec₁ α) (log : QueryLog (spec₁ ++ₒ spec₂)) :
+  simulate (loggingOracle (spec := spec₁ ++ₒ spec₂)) log oa = do
+    let ⟨a, log_oa⟩ ← simulate (loggingOracle (spec := spec₁)) ∅ oa
+    return (a, log.append (QueryLog.inl log_oa)) := by
+  simp [liftM_eq_liftComp, bind_pure_comp]
+  sorry
+
+theorem inr_eq (oa : OracleComp spec₂ α) (log : QueryLog (spec₁ ++ₒ spec₂)) :
+  simulate (loggingOracle (spec := spec₁ ++ₒ spec₂)) log oa = do
+    let ⟨a, log_oa⟩ ← simulate (loggingOracle (spec := spec₂)) ∅ oa
+    return (a, log.append (QueryLog.inr log_oa)) := by
+  simp [liftM_eq_liftComp, bind_pure_comp]
+  sorry
 
 end loggingOracle
